MultiScalarMul_Abstract_Completeness.ec
@@ -9,116 +9,24 @@ require import MultiScalarMul_Abstract MultiScalarMul_Abstract_Setup AuxResults 
 require import Distr.
 
 
+module UniformU : OutCalls = {
+   proc getU() = {
+     var u_cand;
+     u_cand <$ r_distr;
+     return u_cand;
+   }
+}.
+
+
+(* extra assumption on the algorithm parameters  *)
+axiom completeness_constraints :   forall i, 0 <= i < l
+  =>  
+   0 < `| (2 ^ w - 1) * (1 - i) + 2 ^ w * l | < order
+  /\ 0 < `| (1 - 2 ^ w) * (1 + i) + 2 ^ w * l | < order.
+
+
 op p1 : real = mu r_distr (fun (x : R) => x = idR).
 op p2 P s : real = mu r_distr (fun (x : R) => ! u_check x P s).
-
-lemma incompleteAddLoop_specR_ph argcc argT argic args  :
- phoare [ SimpleComp.incompleteAddLoop : arg = (argcc, argT, argic,  args)
-     ==>  res = incompleteAddLoop l argT args argic argcc ] = 1%r.
-proc.
-while (0 <= jc 
- /\ jc <= l 
- /\ flag = (iteri 
-                  jc 
-                  (fun j (acc : bool * R) => 
-                     (acc.`1 /\ xdiff acc.`2 (argT j (args j argic)) , 
-                      acc.`2 %%% argT j (args j argic))) 
-                  (true, argcc)).`1
- /\ (acc, table, ic,  s) = (argcc, argT, argic, args) 
- /\ vahe =  (iteri jc (fun j (acc : bool * R) => (acc.`1 /\ xdiff acc.`2 (argT j (args j argic)) , acc.`2 %%% argT j (args j argic))) (true, argcc)).`2) (l - jc).
-move => z.
-wp. skip. progress. smt(). smt(). rewrite iteriS. smt().
-   simplify.
-   rewrite /xdiff. 
-pose xxx := (iteri jc{hr}
-     (fun (j : int) (acc0 : bool * R) =>
-        (acc0.`1 /\
-         xof acc0.`2 <> xof (table{hr} j (s{hr} j ic{hr})) && acc0.`2 <> idR,
-         acc0.`2 %%% table{hr} j (s{hr} j ic{hr}))) (true, acc{hr})).
-pose yyy := (iteri jc{hr}
-       (fun (j : int) (acc0 : R) => acc0 %%% table{hr} j (s{hr} j ic{hr}))
-       acc{hr}).     smt().
-rewrite iteriS. smt().
-smt(op_assoc).
-smt().   
-   wp. skip. progress. smt(l_pos). 
-rewrite iteri0. auto. auto.
-rewrite iteri0. auto. auto.
-smt().   
-smt().
-qed.  
-
-
-
-lemma incompleteAddLoop_specR_h argcc argT argic args  :
- hoare [ SimpleComp.incompleteAddLoop : arg = (argcc, argT, argic,  args)
-     ==>  res = incompleteAddLoop l argT args argic argcc ].
-conseq (incompleteAddLoop_specR_ph argcc argT argic args).
-qed.   
-
-
-lemma multm_spec_h argP args argU  :
- hoare [ SimpleComp.multiScalarMulMain_Opt : arg = (argP, args, argU)   
-  ==>  res = multiScalarMul T l (perfect_table_pure argP argU) args (l *** argU) w   ] .
-proc. 
-while (
-  0 <= ic 
-  /\ ic <= T
-  /\ (U, table, s) = (argU, (perfect_table_pure argP argU), args) 
-  /\ (flag , acc) = multiScalarMul ic l ((perfect_table_pure argP argU)) args (l *** argU) w
- ) .
-
-wp.
-ecall (incompleteAddLoop_specR_h acc (perfect_table_pure argP argU) ic args).
-ecall (doublewtimes_spec acc w). 
-skip.
-progress. smt(w_pos).
-smt(). smt().
-rewrite /multiScalarMul.
-rewrite iteriS. smt().
-smt().
-wp. skip. progress. smt(T_pos).   
-rewrite /multiScalarMul. rewrite iteri0.
-auto. auto. 
-have -> : T = ic0. smt(T_pos).
-rewrite - H2.
- smt().
-qed. 
-
-
-lemma multm_spec_ph argP args argU  :
- phoare [ SimpleComp.multiScalarMulMain_Opt : arg = (argP, args, argU)   
-  ==>  res = multiScalarMul T l (perfect_table_pure argP argU) args (l *** argU) w ]  = 1%r.
-phoare split ! 1%r 0%r. auto.
-   proc. wp.
-while (table = (perfect_table_pure argP argU) /\ s = args) (T - ic). progress.
-wp.
-exists* acc, table, ic, s.
-elim*. move => accV tableV icV sV.
-call (incompleteAddLoop_specR_ph (2 ^ w *** accV) (perfect_table_pure argP argU) icV args).
-call (doublewtimes_spec_ph accV MultiScalarMul_Abstract.w).
-skip.  progress. smt(w_pos).  smt().
-wp. progress.
-auto. smt(). hoare.
-apply multm_spec_h. 
-qed.
-
-
-
-lemma compl_I_equiv : 
- equiv [ SimpleComp.multiScalarMul_Fun ~
-         MultiScalarMul(UniformU).run
-     : ={arg} ==> res{1}.`1 = res{2}.`1 ].
-proc.
-inline UniformU.getU. 
-
-seq 1 1 : (#pre /\ u_cand{1} = u_cand0{2}).
-    rnd. skip. progress.
-inline SimpleComp.multiScalarMulMain_Opt_Corrected.
-wp.    
-ecall {2} (multm_spec_ph P{2} s{2} u_cand{2}).
-wp. skip. progress.   
-qed.
 
 
 lemma compl_flags P s &m : 
@@ -133,7 +41,7 @@ qed.
 
 
 lemma compl_II_equiv P s &m :
-     Pr[ SimpleComp.multiScalarMul_Fun2(P,s) @&m : !res.`1 ]
+     Pr[ SimpleComp.multiScalarMul_Functional(P,s) @&m : !res.`1 ]
      = Pr[ MultiScalarMul(UniformU).run_perfect(P,s) @&m : !res.`1 ].
 byequiv (_: _ ==> res{1}.`1 = res{2}.`1).
 proc.
@@ -143,19 +51,13 @@ seq 1 1 : (#pre /\ u_cand{1} = u_cand0{2}).
 inline SimpleComp.multiScalarMulMain_Perfect.
 wp.
  exists* P{2}, s{2} , u_cand0{2}. elim*. move => argP argS argU.
-call {2} (multm_spec_ph2 argP argS argU T). smt(T_pos).
+call {2} (multm_spec_ph2 argP argS argU T). smt(param_pos).
 wp. skip. progress. auto. smt().
 qed.
 
-    (*  *)
-axiom completeness_constraints :   forall i, 0 <= i < l
-  =>  
-   0 < `| (2 ^ w - 1) * (1 - i) + 2 ^ w * l | < order
-  /\ 0 < `| (1 - 2 ^ w) * (1 + i) + 2 ^ w * l | < order.
-
 
 lemma completeness_I argP args :
-  phoare [ SimpleComp.multiScalarMul_Fun2 :
+  phoare [ SimpleComp.multiScalarMul_Functional :
       arg = (argP , args) ==> !res.`1 ] 
             <= ((p2 argP args) + (T%r * (l%r * (p1 + p1)))).
 proc.
@@ -168,8 +70,7 @@ rewrite mu_split. simplify.
 apply mu_split_q.
 apply kkkk. smt().
 auto.
-rewrite /multiScalarMul_Complete.
-
+rewrite /multiScalarMulLoop.
   have -> : (fun (x : R) =>
      ! (iteri T
           (fun (i : int) (acc : bool * R) =>
@@ -186,16 +87,12 @@ rewrite /multiScalarMul_Complete.
                  (2 ^ w *** myacc ) in (acc.`1 /\ r.`1, r.`2))
           (true, l *** x)).`1).
 apply fun_ext. move => x.
-
-
-
  rewrite   (iteriG (fun (x : bool * R) => x.`1) (fun (x : bool * R) => x.`2)
    (fun (i : int) (acc1 : bool ) (acc2 : R) =>
          let r =
            completeAddLoop l (perfect_table_pure P{hr} x) s{hr} i
              (2 ^ w *** acc2) in (acc1 /\ r.`1, r.`2)) T _ (true, l *** x)  ).
-smt(T_pos). simplify.
-
+smt(param_pos). simplify.
   pose f1 := (fun (i : int) (acc : bool * R) =>
          (acc.`1 /\
           (completeAddLoop l (perfect_table_pure P{hr} x) s{hr} i
@@ -222,9 +119,7 @@ smt(T_pos). simplify.
             (2 ^ w *** (gg s{hr} P{hr} i x))).`1,
          (completeAddLoop l (perfect_table_pure P{hr} x) s{hr} i
             (2 ^ w *** (gg s{hr} P{hr} i x))).`2)).
-
  rewrite (eq_iteri f1 f2 T _ _).
-
 progress.
  (* apply fun_ext. move => z. apply fun_ext. move => zz. progress. *)
 rewrite /f1 /f2.      
@@ -236,15 +131,13 @@ rewrite /f1 /f2.
             (completeAddLoop l (perfect_table_pure P{hr} x) s{hr} i0
                (2 ^ w *** acc0.`2)).`2)) (true, l *** x)).`2 = gg s{hr} P{hr} i x. 
 rewrite (muleqsimp2 i s{hr} x P{hr}).  auto.
-
       auto. auto. auto.
 apply (iteri_ub3 (fun (x : R) => l *** x)   
         (fun x i => completeAddLoop l (perfect_table_pure P{hr} x) s{hr} i
                (2 ^ w *** (gg s{hr} P{hr} i x) )) r_distr T (l%r * (p1 + p1)) _ ).  
 simplify.
 move => i.
-rewrite /completeAddLoop. simplify.
-             
+rewrite /completeAddLoop. simplify.            
 have -> : (fun (r : R) =>
      ! (iteri l
           (fun (j : int) (acc : bool * R) =>
@@ -268,7 +161,7 @@ apply fun_ext. move => r.
  rewrite   (iteriG (fun (x : bool * R) => x.`1) (fun (x : bool * R) => x.`2)
    (fun (j : int) (acc1 : bool) (acc2 : R) =>
         (acc1 /\ xdiff acc2 (perfect_table_pure P{hr} r j (s{hr} j i)),
-         acc2 +++ perfect_table_pure P{hr} r j (s{hr} j i))) l _ (true, 2 ^ w *** gg s{hr} P{hr} i r)  ). smt(l_pos). simplify. 
+         acc2 +++ perfect_table_pure P{hr} r j (s{hr} j i))) l _ (true, 2 ^ w *** gg s{hr} P{hr} i r)  ). smt(param_pos). simplify. 
 
  pose f1 := (fun (i0 : int) (acc : bool * R) =>
          (acc.`1 /\
